disk-betree/BucketsLib.dfy
@@ -1,0 +1,264 @@
+include "PivotsLib.dfy"
+include "Message.dfy"
+include "../lib/maps.dfy"
+
+module BucketsLib {
+  import opened PivotsLib
+  import opened Lexicographic_Byte_Order
+  import opened ValueMessage
+  import opened Maps
+  import opened Sequences
+
+  type Bucket = map<Key, Message>
+  type BucketList = seq<Bucket>
+
+  predicate {:opaque} WFBucket(bucket: Bucket)
+  {
+    && (forall key | key in bucket :: bucket[key] != IdentityMessage())
+  }
+
+  predicate WFBucketAt(bucket: Bucket, pivots: PivotTable, i: int)
+  requires WFPivots(pivots)
+  {
+    && (forall key | key in bucket :: bucket[key] != IdentityMessage())
+    && (forall key | key in bucket :: Route(pivots, key) == i)
+  }
+
+  predicate WFBucketList(blist: BucketList, pivots: PivotTable)
+  {
+    && WFPivots(pivots)
+    && |blist| == |pivots| + 1
+    && (forall i | 0 <= i < |blist| :: WFBucketAt(blist[i], pivots, i))
+  }
+
+  function BucketGet(bucket: Bucket, key: Key) : Message
+  {
+    if key in bucket then bucket[key] else IdentityMessage()
+  }
+
+  function BucketListGet(blist: BucketList, pivots: PivotTable, key: Key) : Message
+  requires WFBucketList(blist, pivots)
+  {
+    BucketGet(blist[Route(pivots, key)], key)
+  }
+
+  function BucketInsert(bucket: Bucket, key: Key, msg: Message) : Bucket
+  {
+    var msg := Merge(msg, BucketGet(bucket, key));
+    if msg == IdentityMessage() then
+      MapRemove1(bucket, key)
+    else
+      bucket[key := msg]
+  }
+
+  function BucketListInsert(blist: BucketList, pivots: PivotTable, key: Key, msg: Message) : BucketList
+  requires WFBucketList(blist, pivots)
+  {
+    var i := Route(pivots, key);
+    blist[i := BucketInsert(blist[i], key, msg)]
+  }
+
+  function BucketListItemFlush(child: Bucket, pivots: PivotTable, parent: Bucket, i: int) : Bucket
+  requires WFPivots(pivots)
+  {
+    map key
+    | && (key in (child.Keys + parent.Keys)) // this is technically redundant but allows Dafny to figure out that the domain is finite
+      && Route(pivots, key) == i
+      && Merge(BucketGet(parent, key), BucketGet(child, key)) != IdentityMessage()
+    :: Merge(BucketGet(parent, key), BucketGet(child, key))
+  }
+
+  function BucketListFlush'(blist: BucketList, pivots: PivotTable, parent: Bucket, i: int) : BucketList
+  requires WFBucketList(blist, pivots)
+  requires 0 <= i <= |blist|
+  {
+    if i == 0 then [] else (
+      BucketListFlush'(blist, pivots, parent, i-1) + [BucketListItemFlush(blist[i-1], pivots, parent, i-1)]
+    )
+  }
+
+  function BucketListFlush(blist: BucketList, pivots: PivotTable, parent: Bucket) : BucketList
+  requires WFBucketList(blist, pivots)
+  {
+    BucketListFlush'(blist, pivots, parent, |blist|)
+  }
+
+  function JoinBucketList(buckets: seq<Bucket>) : (bucket : Bucket)
+  {
+    if |buckets| == 0 then map[] else MapUnion(JoinBucketList(DropLast(buckets)), Last(buckets))
+  }
+
+  function SplitBucketOnPivots(bucket: Bucket, pivots: seq<Key>) : (buckets: BucketList)
+  ensures |buckets| == |pivots| + 1
+  {
+    if |pivots| == 0 then (
+      [bucket]
+    ) else (
+      var l := map key | key in bucket && Keyspace.lt(key, Last(pivots)) :: bucket[key];
+      var r := map key | key in bucket && Keyspace.lte(Last(pivots), key) :: bucket[key];
+
+      SplitBucketOnPivots(l, DropLast(pivots)) + [r]
+    )
+  }
+
+  ///// Splitting stuff
+
+  function SplitBucketLeft(bucket: Bucket, pivot: Key) : Bucket
+  {
+    map key | key in bucket && Keyspace.lt(key, pivot) :: bucket[key]
+  }
+
+  function SplitBucketRight(bucket: Bucket, pivot: Key) : Bucket
+  {
+    map key | key in bucket && Keyspace.lte(pivot, key) :: bucket[key]
+  }
+
+  function SplitBucketListLeft(blist: BucketList, pivots: PivotTable, cLeft: int, key: Key) : BucketList
+  requires WFBucketList(blist, pivots)
+  requires CutoffForLeft(pivots, key) == cLeft
+  {
+    blist[.. cLeft] + [SplitBucketLeft(blist[cLeft], key)]
+  }
+
+  function SplitBucketListRight(blist: BucketList, pivots: PivotTable, cRight: int, key: Key) : BucketList
+  requires WFBucketList(blist, pivots)
+  requires CutoffForRight(pivots, key) == cRight
+  {
+    [SplitBucketRight(blist[cRight], key)] + blist[cRight + 1 ..]
+  }
+
+  lemma WFSplitBucketLeft(bucket: Bucket, pivot: Key, pivots: seq<Key>, i: int)
+  requires 0 <= i <= |pivots|
+  requires WFPivots(pivots)
+  requires WFBucketAt(bucket, pivots, i)
+  ensures WFPivots(pivots[.. i])
+  ensures WFBucketAt(SplitBucketLeft(bucket, pivot), pivots[.. i], i)
+  {
+    WFSlice(pivots, 0, i);
+    forall key | key in SplitBucketLeft(bucket, pivot)
+    ensures Route(pivots[.. i], key) == i
+    {
+      RouteIs(pivots[.. i], key, i);
+    }
+  }
+
+  lemma WFSplitBucketRight(bucket: Bucket, pivot: Key, pivots: seq<Key>, i: int)
+  requires 0 <= i <= |pivots|
+  requires WFPivots(pivots)
+  requires WFBucketAt(bucket, pivots, i)
+  ensures WFPivots(pivots[i ..])
+  ensures WFBucketAt(SplitBucketRight(bucket, pivot), pivots[i ..], 0)
+  {
+    WFSuffix(pivots, i);
+    forall key | key in SplitBucketRight(bucket, pivot)
+    ensures Route(pivots[i ..], key) == 0
+    {
+      RouteIs(pivots[i ..], key, 0);
+    }
+  }
+
+  lemma WFSplitBucketListLeft(blist: BucketList, pivots: PivotTable, cLeft: int, key: Key)
+  requires WFBucketList(blist, pivots)
+  requires CutoffForLeft(pivots, key) == cLeft
+  ensures WFBucketList(SplitBucketListLeft(blist, pivots, cLeft, key), pivots[.. cLeft])
+
+  lemma WFSplitBucketListRight(blist: BucketList, pivots: PivotTable, cRight: int, key: Key)
+  requires WFBucketList(blist, pivots)
+  requires CutoffForRight(pivots, key) == cRight
+  ensures WFBucketList(SplitBucketListRight(blist, pivots, cRight, key), pivots[cRight ..])
+
+  // This is useful for proving NodeHasWFBuckets(node')
+  // for indices over the given interval [a, b],
+  // assuming we already know the buckets and pivots come from some other
+  // well-formed node (possibly shifted by the amount d).
+  lemma BucketListHasWFBucketAtIdenticalSlice(
+      blist: BucketList, pivots: PivotTable, blist': BucketList, pivots': PivotTable, a: int, b: int, d: int)
+  requires WFBucketList(blist, pivots)
+  requires WFPivots(pivots')
+  requires |pivots'| + 1 == |blist'|
+  requires 0 <= a
+  requires b < |blist'|
+  requires a-d >= 0
+  requires b-d < |blist|
+  requires forall i | a <= i <= b :: blist'[i] == blist[i-d]
+  requires forall i | a <= i < b :: pivots'[i] == pivots[i-d]
+  requires b >= a && b < |pivots'| ==> (
+      || (b-d < |pivots| && pivots'[b] == pivots[b-d])
+      || (forall key | key in blist'[b] :: Keyspace.lt(key, pivots'[b]))
+    )
+  requires b >= a && a-1 >= 0 ==> (
+      || (a-1-d >= 0 && pivots'[a-1] == pivots[a-1-d])
+      || (forall key | key in blist'[a] :: Keyspace.lte(pivots'[a-1], key))
+    )
+  ensures forall i | a <= i <= b :: WFBucketAt(blist'[i], pivots', i)
+  /*{
+    forall i | a <= i <= b
+    ensures NodeHasWFBucketAt(node', i)
+    {
+      assert NodeHasWFBucketAt(node, i - d);
+      forall key | key in node'.buckets[i]
+      {
+        Pivots.RouteIs(node'.pivotTable, key, i);
+      }
+    }
+  }*/
+
+  ///// Other lemmas
+
+  lemma JoinBucketsSplitBucketOnPivotsCancel(bucket: Bucket, pivots: seq<Key>)
+  requires WFPivots(pivots)
+  requires WFBucket(bucket)
+  ensures WFBucketList(SplitBucketOnPivots(bucket, pivots), pivots)
+  ensures JoinBucketList(SplitBucketOnPivots(bucket, pivots)) == bucket
+  /*
+  {
+    if |pivots| == 0 {
+    } else {
+      var l := map key | key in bucket && Keyspace.lt(key, Last(pivots)) :: bucket[key];
+      var r := map key | key in bucket && Keyspace.lte(Last(pivots), key) :: bucket[key];
+
+      var bucketsPref := SplitBucketOnPivots(DropLast(pivots), l);
+      Pivots.WFSlice(pivots, 0, |pivots| - 1);
+      SplitBucketOnPivotsCorrect(DropLast(pivots), l, bucketsPref);
+
+      forall i | 0 <= i < |buckets|
+      ensures WFBucket(buckets[i], pivots, i)
+      {
+        if i < |buckets| - 1 {
+          assert WFBucket(bucketsPref[i], DropLast(pivots), i);
+          forall key | key in buckets[i] ensures Pivots.Route(pivots, key) == i
+          {
+            assert Pivots.Route(DropLast(pivots), key) == i;
+            assert buckets[i] == bucketsPref[i];
+            assert key in bucketsPref[i];
+            assert key in l;
+            Pivots.RouteIs(pivots, key, i);
+          }
+          assert WFBucket(buckets[i], pivots, i);
+        } else {
+          forall key | key in buckets[i] ensures Pivots.Route(pivots, key) == i
+          {
+            Pivots.RouteIs(pivots, key, i);
+          }
+          assert WFBucket(buckets[i], pivots, i);
+        }
+      }
+    }
+  }
+  */
+
+  lemma WFJoinBuckets(buckets: seq<Bucket>)
+  ensures WFBucket(JoinBucketList(buckets))
+  /*
+  {
+    if |buckets| == 0 {
+    } else {
+      JoinBucketsNoIdentity(DropLast(buckets));
+    }
+  }
+  */
+
+  lemma WFBucketListFlush(blist: BucketList, pivots: PivotTable, parent: Bucket)
+  requires WFBucketList(blist, pivots)
+  ensures WFBucketList(BucketListFlush(blist, pivots, parent), pivots)
+}
